lunarlander_sl/BigStepContinuous.thy
@@ -239,6 +239,15 @@ theorem Valid_ode_sp:
   apply (auto simp add: entails_def)
   using entails_mp by (simp add: entails_tassn_def)
 
+theorem Valid_ode_sp2:
+  assumes "b st"
+  shows "\<Turnstile> {\<lambda>s. P s}
+              Cont ode b
+            {\<lambda>s t. \<exists>s'. (P s' @\<^sub>t ODE\<^sub>t s' ode b s) t}"
+  apply (rule Valid_weaken_pre)
+   prefer 2 apply (rule Valid_ode')
+  by (auto simp add: entails_def magic_wand_assn_def join_assn_def)  
+
 theorem Valid_ode_unique_solution_aux:
   assumes
     "d > 0" "ODEsol ode p d" "\<forall>t. t \<ge> 0 \<and> t < d \<longrightarrow> b (p t)"
@@ -246,12 +255,12 @@ theorem Valid_ode_unique_solution_aux:
     "local_lipschitz {- 1<..} UNIV (\<lambda>(t::real) v. ODE2Vec ode (vec2state v))"
     "ODE\<^sub>t st ode b st' tr"
   shows
-    "st' = p d \<and> WaitS\<^sub>t d p ({}, {}) tr"
+    "st' = p d \<and> Wait\<^sub>t d (\<lambda>s. State (p s)) ({}, {}) tr"
 proof -
   have "b st"
     using assms(1,3,5) by auto
   have main: "d2 = d \<and> p d = p2 d2 \<and> (\<lambda>\<tau>\<in>{0..d}. State (p \<tau>)) = (\<lambda>\<tau>\<in>{0..d2}. State (p2 \<tau>)) \<and>
-              WaitS\<^sub>t d p ({}, {}) [WaitBlk d2 (\<lambda>\<tau>. State (p2 \<tau>)) ({}, {})]"
+              Wait\<^sub>t d (\<lambda>s. State (p s)) ({}, {}) [WaitBlk d2 (\<lambda>\<tau>. State (p2 \<tau>)) ({}, {})]"
     if cond: "0 < d2"
        "ODEsol ode p2 d2"
        "(\<forall>t. 0 \<le> t \<and> t < d2 \<longrightarrow> b (p2 t))"
@@ -300,7 +309,7 @@ proof -
       using s8 by (simp add: assms(1) less_eq_real_def)
     have s11: "WaitBlk d (\<lambda>\<tau>. State (p \<tau>)) ({}, {}) = WaitBlk d2 (\<lambda>\<tau>. State (p2 \<tau>)) ({}, {})"
       apply (rule WaitBlk_ext_real) using s7 s8 by auto
-    have s12: "WaitS\<^sub>t d p ({}, {}) [WaitBlk d2 (\<lambda>\<tau>. State (p2 \<tau>)) ({}, {})]"
+    have s12: "Wait\<^sub>t d (\<lambda>s. State (p s)) ({}, {}) [WaitBlk d2 (\<lambda>\<tau>. State (p2 \<tau>)) ({}, {})]"
       unfolding s11[symmetric]
       by (rule wait_assn.intros)
     show ?thesis using s7 s8 s10 s12 by auto
@@ -324,17 +333,18 @@ theorem Valid_ode_unique_solution':
   shows "\<Turnstile>
     {\<lambda>s tr. s = st \<and> Q s tr}
       Cont ode b
-    {\<lambda>s tr. s = p d \<and> (Q st @\<^sub>t WaitS\<^sub>t d p ({}, {})) tr}"
+    {\<lambda>s tr. s = p d \<and> (Q st @\<^sub>t Wait\<^sub>t d (\<lambda>s. State (p s)) ({}, {})) tr}"
 proof -
   have "b st"
     using assms(1,3,5) by auto
-  have *: "ODE\<^sub>t st ode b s tr2 \<Longrightarrow> s = p d \<and> WaitS\<^sub>t d p ({}, {}) tr2" for s tr2
+  have *: "ODE\<^sub>t st ode b s tr2 \<Longrightarrow> s = p d \<and> Wait\<^sub>t d (\<lambda>s. State (p s)) ({}, {}) tr2" for s tr2
     using Valid_ode_unique_solution_aux[OF assms(1-6)] by auto
   show ?thesis
     apply (rule Valid_strengthen_post)
      prefer 2 apply (rule Valid_ode_sp)
     by (auto simp add: \<open>b st\<close> entails_def join_assn_def *)
 qed
+
 
 theorem Valid_ode_exit:
   assumes "\<not> b st"
